error codes

src/frontend/ocaml/parser.mly
@@ -108,7 +108,8 @@ struct_field:
          field_type=t;
          field_array_opt=aopt;
          field_constraint=c;
-         field_size=None
+         field_size=None;
+         field_number=None
         }
     }
 
